papers/116_stefan_rass/Supplementary/Option_S.thy
@@ -37,4 +37,7 @@ qed
 lemma these_id: "None \<notin> A \<Longrightarrow> Option.these A = the ` A" unfolding Option.these_def by fast
 
 
+lemma card_set_option[simp]: "card (set_option x) \<le> 1" by (induction x) auto
+lemma finite_set_option[simp]: "finite (set_option x)" by (induction x) auto
+
 end
